\documentclass[11pt]{article}
\title{Propositions of solutions for \textit{Analysis I} by Terence Tao}
\author{Frédéric Santos}
% General packages:
\usepackage{a4wide}
\usepackage[english]{babel}
\usepackage[utf8]{inputenc} 
\usepackage[T1]{fontenc}
\usepackage{titlesec}
\titlelabel{\thetitle.\quad}
\usepackage{enumitem}
% Fonts and math packages:
\usepackage{lmodern}
\usepackage{amsmath}
\usepackage[matha,mathb]{mathabx}
\usepackage{mbboard}
\usepackage{stmaryrd}
% Macros:
\newcommand{\successor}[1]{#1 \! +\!\!\!+}
% Lemmas:
\usepackage{amsthm}
\newtheorem*{lem}{Lemma}
% Environment:
\newenvironment{exo}[2]{\noindent \textsc{Exercise #1}. ---
  \textit{#2} \vspace{3mm}}

% Begin doc:
\begin{document}
\maketitle

\section{Introduction}
\label{sec:introduction}
No exercises in this chapter.

\section{The natural numbers}
\label{sec:natural-numbers}
\begin{exo}{2.2.1}{Prove that the addition is associative, i.e. that
    for any natural numbers $a, b, c$, we have $(a+b) + c = a + (b+c)$.}

  Let's use induction on $c$ while keeping $a$ and $b$ fixed.
  
  \begin{itemize}
  \item Base case for $c=0$: let's prove that $(a+b)+0 = a+(b+0)$. The
    left hand side is equal to $(a+b)$ according to Lemma 2.2.3. For the
    right hand side, if we apply the same lemma to the $(b+0)$ part,
    we get $a + (b+0) = a+b$. Both sides are equal to $a+b$, and the
    base case is thus done.
  \item Now let's suppose inductively that $(a+b) + c = a + (b+c)$: we
    have to prove that $(a+b) + \successor{c} = a + (b +
    \successor{c})$. Using Lemma 2.2.3 on the right
    hand side leads to $a + \successor{(b+c)}$. Now consider the left
    hand side. Using still the same lemma, we get $(a+b) +
    \successor{c} = \successor{\left((a+b) + c\right)}$. By the
    inductive hypothesis, this is also equal to
    $\successor{\left(a + (b+c)\right)}$. And, using the lemma 2.2.3
    again, this also leads to $a + \successor{b+c}$. Therefore, both
    sides are equal to $a + \successor{b+c}$, and we have closed the
    induction.
  \end{itemize}
\end{exo}

\begin{exo}{2.2.2}{Let $a$ be a positive number. Prove that there
    exists exactly one natural number $b$ such that $\successor{b} =
    a$.}
  
  Let's use induction on $a$.

  \begin{itemize}
  \item Base case for $a=1$: we know that $b=0$ matches this property,
    since $\successor{0} = 1$ by Definition 2.1.3. Furthermore, there
    is only one solution. Suppose that is another natural number $b$
    such that $\successor{b} = 1$. Then, we would have
    $\successor{b} = \successor{0}$, which would imply $b = 0$ by
    Axiom 2.4. The base case is demonstrated.
  \item Let's suppose inductively that there is exactly one natural
    number $b$ such that $\successor{b} = a$. We have to prove that
    there is exactly one natural number $b'$ such that
    $\successor{b'} = \successor{a}$. By the induction hypothesis, and
    taking $b' = \successor{b}$, we have
    $\successor{b'} = \successor{(\successor{b})} = \successor{a}$. So
    there exists a solution, with $b' = \successor{b} = a$. Uniqueness is
    given by Axiom 2.4.: if $\successor{b'} = \successor{a}$, then we
    necessarily have $b'=a$.
  \end{itemize}
\end{exo}

\begin{exo}{2.2.3}{Let $a, b, c$ be natural numbers. Prove the
    following properties of order for natural numbers:}
  \begin{enumerate}[label=\emph{(\alph*)}]
  \item Reflexivity: $a \geq a$. This is true since $a = 0 + a$ by
    Definition 2.2.1. By commutativity of addition, we can also write
    $a = a + 0$. So there is indeed a natural number $n$ (with
    $n=0$) such that $a = a + n$, i.e. $a \geq a$.
  \item Transitivity: if $a \geq b$ and $b \geq c$, then $a \geq
    c$. From the part $a \geq b$, there exists a natural number $n$
    such that $a = b + n$ according to Definition 2.2.11. A similar
    consideration for the part $b \geq c$ leads to $b = c + m$, $m$
    being a natural number. Combining together those two equalities,
    we can write $a = b + n = (c + m) + n = c + (m + n)$ by
    associativity (see Exercise 2.2.1). Then, $n+m$ being a natural
    number\footnote{This is a trivial induction from the definition of
      addition.}, the transitivity is demonstrated.
  \item Anti-symmetry: if $a \geq b$ and $b \geq a$, then $a=b$. From
    the part $a \geq b$, there exists a natural number $n$ such that $a
    = b + n$. Similarly, there exists a natural number $m$ such that $b
    = a + m$. Combining those two equalities leads to $a = b + n = (a +
    m) + n = a + (m + n)$. By cancellation law (Proposition 2.2.6), we
    can conclude that $0 = m + n$. According to Corollary 2.2.9, this
    leads to $m = n = 0$. Therefore, both $m$ and $n$ are null,
    meaning that $a = b + 0 = b$.
  \item Preservation of order: $a \geq b$ iff $a + c \geq b +
    c$. First, let's prove that
    $a+c \geq b+c \Longrightarrow a \geq b$. If $a+c \geq b+c$, there
    exists a natural number $n$ such that $a+c = b+c+n$. By
    cancellation law (Proposition 2.2.6)\footnote{And also
      associativity and commutativity that we do not detail explicitly
      here.}, we conclude that $a = b + n$, i.e. $a\geq b$, thus
    demonstrating the first implication. Conversely, let's suppose
    that $a \geq b$. There exists a natural number $m$ such that
    $a = b + m$. Therefore, $a + c = b+m+c$ for any natural number
    $c$. Still by associativity and commutativity, we can rewrite this
    as $a+c = (b+c) +m$, i.e. $a+c \geq b+c$.
  \item $a < b$ iff $\successor{a} \leq b$. First, let's prove that
    $\successor{a} \leq b \Longrightarrow a < b$. By definition of
    ordering, there exists a natural number $n$ such that
    $b = (\successor{a}) + n$. By definition of addition, we can
    re-write: $b = \successor{(\successor{a} + n)}$. Then, by
    commutativity and yet again by definition of addition,
    $b = \successor{(n + \successor{a})} = (\successor{n}) +
    (\successor{a})$. Thus, there exists a natural number
    $\successor{n}$ such that $b = \successor{n} + a$, which means that
    $b \geq a$. But we still have to prove that $a \neq b$. Let's
    suppose that $a=b$: in this case, by cancellation law, we would
    have $\successor{n} = 0$, which is impossible according to Axiom
    2.3 (0 is not the successor of any natural number). Thus, $a \neq
    b$ et $b \geq a$: we have showed that $a < b$. 

    Conversely, let's prove that
    $a < b \Longrightarrow \successor{a} \leq b$. Starting from that
    strict inequality, there exists a \textit{positive}\footnote{We
      make use here of the statement \textit{(f)} demonstrated
      below. There is no circularity here, since proving \textit{(f)}
      will not make use of \textit{(e)}.} natural number $n$ such that
    $b = a + n$. By Lemma 2.2.10, since $n$ is positive, it has one
    unique antecessor $m$, so that $n$ can be written
    $\successor{m}$. Thus,
    $b = a + (\successor{m}) = \successor{(a + m)} = \successor{(m +
      a)} = m + (\successor{a}) = (\successor{a}) + m$. And, $m$ being
    a natural number, this corresponds to the statement $b \geq a$.
  \item $a < b$ iff $b=a+d$ for some positive number $d$. First, let's
    prove the first implication, $a<b \Longrightarrow b=a+d$ with
    $d \neq 0$. Since $a<b$, we have in particular $a \leq b$, and
    there exists a natural number $d$ such that $b=a+d$. For the sake
    of contradiction, let's suppose that $d=0$. We would have $b=a$,
    which would contradict the condition $a\neq b$ of the strict
    inequality. Thus, $d$ is a positive number, which demonstrates the
    left-to-right implication.

    Conversely, let's suppose that $b = a+d$, with $d \neq 0$. This
    expression gives immediately $a \leq b$. But if $a=b$, by
    cancellation law, this would lead to $0=d$, a contradiction with
    the fact that $d$ is a positive number. Thus, $a\neq b$ and $a
    \leq b$, which demonstrates $a<b$.
  \end{enumerate}
\end{exo}

\begin{exo}{2.2.4}{Demonstrate three lemmas used to prove the
    trichotomy of order for natural numbers.}
  \begin{enumerate}[label=\emph{(\alph*)}]
  \item Show that we have $0 \leq b$ for any natural number $b$. This is obvious
    since, by definition of addition, $0 + b = b$ for any natural
    number $b$. This is precisely the definition of $0 \leq b$.
  \item Show that if $a > b$, then $\successor{a} > b$. If $a > b$,
    then $a = b + d$, $d$ being a positive natural number. Let's
    recall that $\successor{a} = a + 1$. Thus, $\successor{a} = a + 1
    = b + d + 1 = b + (d+1)$ by associativity of
    addition. Furthermore, $d+1$ is a positive natural number (by
    Proposition 2.2.8). Thus, $\successor{a} > b$.
  \item Show that if $a=b$, then $\successor{a}>b$. Once again, let's
    use the fact that $\successor{a} = a+1$. Thus, $\successor{a} =
    a+1 = b+1$, and $1$ is a positive natural number. This is the
    definition of $\successor{a}>b$.
  \end{enumerate}
\end{exo}

\begin{exo}{2.2.5}{Prove the strong principle of induction, formulated
    as follows: Let $m_0$ be a natural number, and let $P(m)$ be a
    property pertaining to an arbitrary natural number $m$. Suppose
    that for each $m \geq m_0$, we have the following implication: if
    $P(m')$ is true for all natural numbers $m_0 \leq m' < m$, then
    $P(m)$ is also true. (In particular, this means that $P(m_0)$ is
    true, since in this case the hypothesis is vacuous.) Then we can
    conclude that $P(m)$ is true for all natural numbers
    $m \geq m_0$.}

  First let's introduce a small lemma (similar to Proposition
  2.2.12\textit{(e)}).

  \begin{lem}
    For any natural number $a$ and $b$, $a<\successor{b}$ iff $a\leq
  b$.
  \end{lem}
  \begin{proof}
    If $a < \successor{b}$, then $\successor{b} = a+n$ for a given
    positive natural $n$. By Lemma 2.2.10, there exists one natural
    number $m$ such as $n = \successor{m}$. Thus $\successor{b} = a +
    \successor{m}$, which can be rewritten $\successor{b} =
    \successor{(a+m)}$ by Lemma 2.2.3\footnote{We could also rewrite
      $b+1 = a + m + 1$ and then use the cancellation law.}. By Axiom
    2.4., this is equivalent to $b = a+n$, which can also be written
    $a \leq b$.
    
    Conversely, if $a \leq b$, there exists a natural number $m$
    such as $b = a+m$. Thus, $\successor{b} = \successor{(a+m)} =
    a + (\successor{m})$ by Definition of addition
    (2.2.1). And, $\successor{m}$ being a positive
    number, this means that $b > a$ according to Proposition
    2.2.12\textit{(f)}.
  \end{proof}

  Now we can prove the main proposition. Let $Q(n)$ be the property
  ``$P(m)$ is true for all $m$ such that $m_0 \leq m < n$''. Let's
  induct on $n$.

  \begin{itemize}
  \item (Although this is not necessary,) we could consider two types
    of base cases. If $n < m_0$, $Q(n)$ is the proposition ``$P(m)$ is
    true for all $m$ such that $m_0 \leq m < n$'', but there is no
    such natural number $m$. Thus, $Q(n)$ is vacuously true. If
    $n = m_0$, $P(m_0)$ is true by hypothesis, thus $Q(m_0)$ is also
    true.
  \item Now let's suppose inductively that $Q(n)$ is true, and show
    that $Q(\successor{n})$ is also true. If $Q(n)$ is true, $P(m)$ is
    true for all $m$ such that $m_0 \leq m < n$. By hypothesis, this
    implies that $P(n)$ is true. Thus, $P(m)$ is true for any natural
    number $m$ such that $m_0 \leq m \leq n$, i.e. such that $m_0 \leq
    m < \successor{n}$ according to the lemma introduced above. This
    is precisely $Q(\successor{n})$, and this closes the induction.
  \end{itemize}
  Thus, $Q(n)$ is true for all natural numbers $n$, which means in
  particular that $P(m)$ is true for any natural number $m \geq
  m_0$. This demonstrates the principle of strong induction.
\end{exo}

\bigskip
\begin{exo}{2.2.6}{Let $n$ be a natural number, and let $P(m)$ be a
    property pertaining to the natural numbers such that whenever
    $P(\successor{m})$ is true, then $P(m)$ is true. Suppose that
    $P(n)$ is also true. Prove that $P(m)$ is true for all natural
    numbers $m \leq n$; this is known as the \emph{principle of
      backwards induction}.}
  
  Terence Tao suggests to use induction on $n$. So let $Q(n)$ be the
  following property: ``if $P(n)$ is true, then $P(m)$ is true for all
  $m \leq n$. The goal is to prove $Q(n)$ for all natural numbers $n$.

  \begin{itemize}
  \item Base case $n = 0$: here, $Q(n)$ means that if $P(0)$ is true,
    then $P(m)$ is true for any $m \leq 0$. By Definition 2.2.11, if
    $m \leq 0$, there exists a natural number $d$ such that $0 = m +
    d$. But, by Corollary 2.2.9, this implies that both $m = 0$ and $d
    = 0$. Thus, the only number $m$ such that $m \leq 0$ is 0
    itself. Therefore, $Q(0)$ is simply the tautology ``if $P(0)$ is
    true, then $P(0)$ is true''--- a statement that we can safely
    accept. The base case is the, demonstrated.
  \item Let's suppose inductively that $Q(n)$ is true: we must show
    that $Q(\successor{n})$ is also true. If $P(\successor{n})$ is
    true, then by definition of $P$, $P(n)$ is also true. Then, by
    induction hypothesis, $P(m)$ is true for all $m \leq n$. We have
    showed that $P(\successor{n})$ implies $P(m)$ for all
    $m \leq \successor{n}$\footnote{Actually, we use here yet another
      lemma, similar to the one introduced for the previous
      exercise. We use the fact that $m \leq \successor{n}$ is
      equivalent to $m = \successor{n}$ or $m \leq n$, which is easy
      to prove, but is not part of the ``standard'' results presented
      in the textbook.}, which is precisely $Q(\successor{n})$. This
    closes the induction.
  \end{itemize}
\end{exo}

\begin{exo}{2.3.1}{Show that multiplication is commutative, i.e., if
    $n$ and $m$ are natural numbers, show that $n \times m = m \times
    n$.}

  We will use an induction of $n$ while keeping $m$ fixed. However,
  this is not a trivial result, and even the base case is not
  straightforward. We will first introduce some lemmas.

  \begin{lem}
    For any natural number $n$, $n \times 0 = 0$.
  \end{lem}

  \begin{proof}
    Let's induct on $n$.
    For the base case $n=0$, we know by Definition 2.3.1 of
    multiplication that $0 \times 0 = 0$, since $0 \times m = 0$ for
    any natural number $m$.

    Now let's suppose that $n \times 0 = 0$. Thus, $\successor{n}
    \times 0 = (n \times 0) + 0$ by Definition 2.3.1. But by induction
    hypothesis, $n \times 0 = 0$, so that $\successor{n} \times 0 = 0
    + 0 = 0$. This closes the induction.
  \end{proof}

  \begin{lem}
    For all natural numbers $m$ and $n$, we have $m \times \successor{n} = (m
    \times n) + m$.
  \end{lem}

  \begin{proof}
    Let's induct on $m$. The base case $m=0$ is easy to prove: $0
    \times \successor{n} = 0$ by Definition 2.3.1 of multiplication, and $(0
    \times n) + 0 = 0$.

    Now suppose inductively that
    $m \times \successor{n} = (m \times n) + m$, and we must show that
    \begin{equation}
      \label{eq:proof_lemma_231}
      \successor{m} \times \successor{n} = (\successor{m} \times n) +
      \successor{m}
    \end{equation}

    We begin by the left hand side: by Definition
    2.3.1,
    $\successor{m} \times \successor{n} = (m \times \successor{n}) +
    \successor{n}$. By induction hypothesis, this is equal to
    $(m \times n) + m + \successor{n}$.

    Then, apply the definition of multiplication to the right hand
    side:
    $(\successor{m} \times n) + \successor{m} = (m \times n) + n +
    \successor{m}$. The Lemma 2.2.3 and the commutativity of addition
    leads to
    $(m \times n) + n + \successor{m} = (m \times n) + \successor{(n +
      m)} = (m \times n) + \successor{(m + n)} = (m \times n) + m +
    \successor{n}$, which is equal to the left hand side.

    Thus, both sides of equation \eqref{eq:proof_lemma_231} are equal,
    and we can close the induction.
  \end{proof}
  
  Now it is easier to prove the main result ($n \times m = m \times
  n$), by an induction on $n$.

  \begin{itemize}
  \item Base case $n = 0$: we already know by Definition 2.3.1 that $0
    \times m = 0$. The first lemma introduced in this exercise also
    provides $m \times 0 = 0$. Thus, the base case is proven, since $0
    \times m = m \times 0 \; (= 0)$.
  \item Now we suppose inductively that $n \times m = m \times n$, and
    we must prove that:
    \begin{equation}
      \label{eq:recurr_commutativity_of_multiplication}
      \successor{n} \times m = m \times \successor{n}
    \end{equation}
    By Definition 2.3.1 of multiplication, the left hand side is equal
    to $(n \times m) + m$.

    Using the lemma introduced above, the right hand side is equal to
    $(m \times n) + m$. By induction hypothesis, this is also equal to
    $(n \times m) + m$, which closes the induction.
  \end{itemize}  
\end{exo}
\end{document}
